\begin{eqnarray*}
&&-\int_{-\infty}^{\infty} p(x)\ln p(x) {\rm d}x + \lambda _1 \left( \int_{-\infty}^{\infty} p(x){\rm d}x - 1 \right) \\
&&\lambda _2 \left( \int_{-\infty}^{\infty} xp(x){\rm d}x - \mu \right)  + \lambda _3 \left( \int_{-\infty}^{\infty} (x-\mu)^2 p(x){\rm d}x - \sigma ^2 \right)
\end{eqnarray*}
\begin{equation*}
 p(x) = \exp \{-1 + \lambda _1 + \lambda _2 x + \lambda _3 (x-\mu) ^2\}
\end{equation*}
\begin{equation*}
p(x) = \frac{1}{(2\pi \sigma^2)^{1/2}} \exp \left\{ - \frac{(x-\mu)^2}{2\sigma ^2} \right\}
\end{equation*}
